src/CSL/ThreadReg.v
@@ -1,0 +1,171 @@
+From iris.algebra Require Export auth functions csum.
+Require Export CSL.WeakestPre CSL.Lifting CSL.Counting.
+Require Import Helpers.RelationTheorems.
+From iris.proofmode Require Export tactics.
+From RecoveryRefinement Require Export Lib.
+
+Class tregG Σ := TRegG {
+                     treg_counter_inG :> inG Σ (csumR countingR (authR (optionUR (exclR unitC))));
+                     treg_name: gname
+                   }.
+Arguments treg_name {_}.
+
+Section thread_reg.
+  Context `{tr: tregG Σ}.
+  Definition Registered :=
+    own (treg_name tr) (Cinl (Count (-1)%Z)).
+  Definition AllDone :=
+    own (treg_name tr) (Cinr (◯ (Excl' tt))).
+  Lemma AllDone_Register_excl:
+    AllDone -∗ Registered -∗ False.
+  Proof. iIntros "Had Hreg". iDestruct (own_valid_2 with "Had Hreg") as %[]. Qed.
+End thread_reg.
+
+
+Definition thread_count_interp {Σ} {tr: tregG Σ} :=
+  λ n, (match n with
+         | 1 => own (treg_name tr) (Cinl (Count 1)) ∨ own (treg_name tr) (Cinr (● (Excl' tt)))
+         | _ => own (treg_name tr) (Cinl (Count n))
+         end)%I.
+
+Module Reg_wp.
+Section Reg_wp.
+Context {OpT} {Λ: Layer OpT} `{IRIS: irisG OpT Λ Σ}.
+Context `{!tregG Σ}.
+
+Lemma fst_lift_puts_inv {A B} f (n1: A) (σ1 : B) n2 σ2 t :
+  fst_lift (puts f) (n1, σ1) (Val (n2, σ2) t) →
+  n2 = f n1 ∧
+  σ2 = σ1 ∧
+  t = tt.
+Proof.
+  intros [Hput ?].
+  inversion Hput; subst; auto.
+Qed.
+
+Context (Interp: OpState Λ → iProp Σ).
+Context (Hinterp1: ∀ n σ, state_interp (n, σ) -∗ thread_count_interp n ∗ Interp σ).
+Context (Hinterp2: ∀ n σ, thread_count_interp n ∗ Interp σ -∗ state_interp (n, σ)).
+
+Lemma wp_spawn {T} s E (e: proc _ T) Φ :
+  ▷ Registered
+    -∗ ▷ (Registered -∗ WP (let! _ <- e; Unregister)%proc @ s; ⊤ {{ _, True }})
+    -∗ ▷ ( Registered -∗ Φ tt)
+    -∗ WP Spawn e @ s; E {{ Φ }}.
+Proof.
+  iIntros "Hreg He HΦ".
+  iApply wp_lift_atomic_step.
+  { auto. }
+  iIntros ((n, σ)) "Hown".
+  iModIntro. iSplit.
+  { destruct s; intuition. iPureIntro. eapply spawn_non_errorable. }
+  iIntros (e2 (n', σ2) ? Hstep) "!>".
+  destruct Hstep as ([]&(?&?)&Hput&Hpure).
+  inversion Hpure. subst.
+  apply fst_lift_puts_inv in Hput as (?&?&?); subst.
+
+  iDestruct (Hinterp1 with "Hown") as "(Hown&Hrest)".
+  iAssert (own (treg_name _) (Cinl (Count n)) ∗ Registered)%I
+          with "[Hown Hreg]" as "(Hown&Hreg)".
+  {
+    destruct (decide (n = 1)) as [->|]; last first.
+    {  destruct n as [|[|n]]; try lia; iFrame. }
+    iDestruct "Hown" as "[Hown|Hown]"; first by iFrame.
+    iDestruct (own_valid_2 with "Hown Hreg") as %[].
+  }
+  iAssert (own (treg_name _) (Cinl (Count (S n))) ∗ Registered)%I
+          with "[Hown]" as "(Hown&Hreg')".
+  {
+    rewrite -own_op Cinl_op counting_op' //=.
+    repeat destruct decide; try lia. replace (S n + (-1))%Z with (n : Z) by lia. done.
+  }
+  iModIntro. simpl. iFrame.
+  iSplitL "Hown Hrest".
+  { iApply Hinterp2. destruct n; iFrame. }
+  iSplitL "Hreg HΦ".
+  { by iApply "HΦ". }
+  rewrite right_id.
+  by iApply "He".
+Qed.
+
+Lemma wp_unregister s E :
+  {{{ ▷ Registered }}} Unregister @ s; E {{{ RET tt; True }}}.
+Proof.
+  iIntros (Φ) ">Hreg HΦ".
+  iApply wp_lift_atomic_step.
+  { auto. }
+  iIntros ((n, σ)) "Hown".
+  iModIntro. iSplit.
+  { destruct s; intuition. iPureIntro. eapply unregister_non_errorable. }
+  iIntros (e2 (n', σ2) ? Hstep) "!>".
+  destruct Hstep as ([]&(?&?)&Hput&Hpure).
+  inversion Hpure. subst.
+  apply fst_lift_puts_inv in Hput as (?&?&?); subst.
+  iDestruct (Hinterp1 with "Hown") as "(Hown&Hrest)".
+
+  iAssert (∃ n', ⌜ n = S n' ⌝ ∗ own (treg_name _) (Cinl (Count n)) ∗ Registered)%I
+          with "[Hown Hreg]" as (n' Heq) "(Hown&Hreg)".
+  {
+    destruct (decide (n = 1)) as [->|]; last first.
+    {  destruct n as [|[|n]]; try lia.
+       - iDestruct (own_valid_2 with "Hown Hreg") as %[].
+       - iExists (S n). iFrame; eauto.
+    }
+    iExists O. iDestruct "Hown" as "[Hown|Hown]"; first by (iFrame).
+    iDestruct (own_valid_2 with "Hown Hreg") as %[].
+  }
+  subst.
+  iAssert (own (treg_name _) (Cinl (Count n')))%I
+          with "[Hown Hreg]" as "Hown".
+  {
+    iCombine "Hown Hreg" as "Hown".
+    rewrite Cinl_op counting_op' //=.
+    repeat destruct decide; try lia. replace (S n' + (-1))%Z with (n' : Z) by lia. done.
+  }
+  iModIntro. simpl. iFrame. iSplitL "Hown Hrest".
+  { iApply Hinterp2. destruct n' as [|[|n']]; iFrame. }
+  rewrite right_id.
+  by iApply "HΦ".
+Qed.
+
+Lemma wp_wait s E :
+  {{{ ▷ Registered }}} Wait @ s; E {{{ RET tt; AllDone }}}.
+Proof.
+  iIntros (Φ) ">Hreg HΦ".
+  iApply wp_lift_atomic_step.
+  { auto. }
+  iIntros ((n, σ)) "Hown".
+  iModIntro. iSplit.
+  { destruct s; intuition. iPureIntro. eapply wait_non_errorable. }
+  iIntros (e2 (n', σ2) ? Hstep) "!>".
+  destruct Hstep as ([]&(?&?)&Hput&Hpure).
+  inversion Hpure. subst.
+  inversion Hput as [Hsuch Heq]. subst.
+  inversion Hsuch; subst.
+  iDestruct (Hinterp1 with "Hown") as "(Hown&Hrest)".
+
+  iAssert (own (treg_name _) (Cinl (Count 1)) ∗ Registered)%I
+          with "[Hown Hreg]" as "(Hown&Hreg)".
+  {
+    iDestruct "Hown" as "[Hown|Hown]"; first by (iFrame).
+    iDestruct (own_valid_2 with "Hown Hreg") as %[].
+  }
+  subst.
+  iAssert (own (treg_name _) (Cinl (Count O)))%I
+          with "[Hown Hreg]" as "Hown".
+  {
+    iCombine "Hown Hreg" as "Hown".
+    rewrite Cinl_op counting_op' //=.
+  }
+  iMod (own_update with "Hown") as "(Hdone&Hown)".
+  { apply cmra_update_exclusive with (y:=Cinr (◯ (Excl' tt)) ⋅ Cinr (● (Excl' tt))) => //=. }
+  iModIntro.
+  iSplitL "Hown Hrest".
+  { iApply Hinterp2; iFrame. }
+  simpl.
+  rewrite right_id.
+  by iApply "HΦ".
+Qed.
+
+End Reg_wp.
+End Reg_wp.
